\section{Singularity solution for droplets with surface tension gradient}
\label{ap:singularity_solution}
At the leading order in droplet volume fraction, the closure problem is equivalent to that of an isolated droplet in an infinite medium \citet{hinch1977averaged}. 
Hence, we consider the problem of an isolated droplet, immersed in an arbitrary quadratic flow without the presence of fluid inertia. 
The disturbances pressure and velocity field are noted $\textbf{u}_{out}$, $\textbf{u}_{in}$, $p_{out}$ and $p_{in}$, for the velocity outside the droplet, the velocity inside the droplet, the pressure outside the droplet and the pressure inside the droplet, respectively. 
The corresponding ``undisturbed field'' are noted $\textbf{u}$ and $p_f$, corresponding to the ensemble averaged mixture velocity and averaged pressure of the continuous phase in the main text. 

Under these hypotheses, in dimensionless form, $\textbf{u}_{out}$, $\textbf{u}_{in}$, $p_i$ and $p_o$ are governed by the Stokes equations, namely, 
\begin{align}
    \div \textbf{u}_{in} &= 0 
    & \div \textbf{u}_{out} &= 0 \\
     \grad^2 \textbf{u}_{in}  &= \grad p_{in} 
    & \grad^2 \textbf{u}_{out} &= \grad p_{out} 
\end{align}
At the surface of the droplet ($r=1$) the condition of continuity of velocity and continuity of the normal stresses read, 
\begin{align}
    \label{eq:vel_jump}
    \textbf{u}_{out} - \textbf{u}_{in} &= 0\\
    % (\textbf{u}_{in}  + \textbf{u} - \textbf{u}_\Gamma)\cdot \textbf{n}
    % = 
    \label{eq:vel_jump2}
    (\textbf{u}_{in}  + \textbf{u}_r)\cdot \textbf{n}
    &= 0\\
    \mathbf{n}\cdot (\textbf{e}_{out} - \lambda \textbf{e}_{in}+\textbf{E} -\lambda\textbf{E} )\cdot (\bm\delta - \textbf{nn})
    &= 
    \textbf{b}\cdot (\bm\delta - \textbf{nn})
    \label{eq:stress_jump}
\end{align}
where $\textbf{u}_r = \textbf{u} - \textbf{u}_p$ corresponds to the velocity of the mixture with respect to the droplet mean velocity. 
We recall that $\textbf{e}_{in/out} = (\grad \textbf{u}_{in/out} + ^\dagger \grad \textbf{u}_{in/out})/2 $ and $\textbf{E} = (\grad \textbf{u} + ^\dagger \grad \textbf{u})/2$, which correspond to the rate of strain inside or around or droplet, and to the ensemble averaged rate of strain, respectively. 
In \ref{eq:stress_jump} the vector \textbf{b} correspond to the dimensionless tangential stress jump across the interface and reads, 
\begin{equation}
    \textbf{b}
    =
    \frac{a \grad \gamma}{2 \mu_f U}
    % \approx (a\grad) Ca^{-1}. 
\end{equation}
Far from the droplet (centered at $\textbf{r}=\textbf{0}$) the velocity and pressure fields satisfy, 
\begin{equation}
    \lim_{r\to \infty}(\textbf{u}_{out},p_{out}) = 0. 
\end{equation}

In general $\textbf{b}$ as well as $\textbf{u}$ are not constant vectors and vary across space as a function of \textbf{r}. 
However, it can be assumed that these quantities are slowly varying functions of space at the scale of a droplet radius, hence we may introduce the simplifications 
\begin{align*}
    \textbf{u}(\textbf{n}) 
    &=  \textbf{u}_r|_{\textbf{r}=0}
    +  \textbf{r} \cdot  \grad\textbf{u}|_{\textbf{r}=0}
    +  \frac{1}{2}\textbf{rr} :  \grad\grad\textbf{u}|_{\textbf{r}=0}
    + \ldots\\
     \textbf{E}(\textbf{n}) 
    &=   \textbf{E}|_{\textbf{r}=0}
    + \textbf{r} \cdot  \grad \textbf{E}|_{\textbf{r}=0}
    + \frac{1}{2}\textbf{rr} :  \grad\grad \textbf{E}|_{\textbf{r}=0}
    + \ldots\\
     \textbf{b}(\textbf{n}) 
    &=   \textbf{b}|_{\textbf{r}=0}
    + \textbf{r} \cdot  \grad \textbf{b}|_{\textbf{r}=0}
    + \frac{1}{2}\textbf{rr} :  \grad\grad \textbf{b}|_{\textbf{r}=0}
    + \ldots
\end{align*}
Note that because $\textbf{b} \sim \grad \gamma$ the tensor: $\grad \textbf{b}$ and $\grad\grad \textbf{b}$ are symmetric tensors. 
Injecting, these expressions into \ref{eq:vel_jump,eq:vel_jump2,eq:stress_jump} one deduce that the velocity and pressure fields are linearly related to $\textbf{u}|_{\textbf{r}=0}$, $\textbf{b}|_{\textbf{r}=0}$, and to the gradients of these vectors. 

According to the linearity of the Stokes equations we deduce that $\textbf{u}_{i/o}$ and $p_{i/o}$  must be linear combination of spherical harmonics proportional to $\textbf{u}|_{\textbf{x}=0}$, $\grad \gamma|_{\textbf{x}=0}$, and their derivatives.
Hence, we can write that the disturbance velocity and pressure fields are given by, 
\begin{align*}
    \begin{pmatrix}
        \textbf{u}_{o}\\
        p_{o}\\
        \textbf{u}_{i}\\
        p_{i}
    \end{pmatrix}
    =
    \begin{pmatrix}
        \textbf{U}_{o}^{(1)} + \textbf{U}_{o}^{(2)}\cdot \grad + \textbf{U}_{o}^{(3)} :\grad\grad &
        \textbf{U}_{o}^\text{(b-1)} + \textbf{U}_{o}^\text{(b-2)}\cdot \grad + \textbf{U}_{o}^\text{(b-3)} :\grad\grad \\
        \textbf{P}_{o}^{(1)} + \textbf{P}_{o}^{(2)}\cdot \grad + \textbf{P}_{o}^{(3)} :\grad\grad &
        \textbf{P}_{o}^\text{(b-1)} + \textbf{P}_{o}^\text{(b-2)}\cdot \grad + \textbf{P}_{o}^\text{(b-3)} :\grad\grad \\
        \textbf{U}_{i}^{(1)} + \textbf{U}_{i}^{(2)}\cdot \grad + \textbf{U}_{i}^{(3)} :\grad\grad &
        \textbf{U}_{i}^\text{(b-1)} + \textbf{U}_{i}^\text{(b-2)}\cdot \grad + \textbf{U}_{i}^\text{(b-3)} :\grad\grad \\
        \textbf{P}_{i}^{(1)} + \textbf{P}_{i}^{(2)}\cdot \grad + \textbf{P}_{i}^{(3)} :\grad\grad &
        \textbf{P}_{i}^\text{(b-1)} + \textbf{P}_{i}^\text{(b-2)}\cdot \grad + \textbf{P}_{i}^\text{(b-3)} :\grad\grad \\
    \end{pmatrix}
    \cdot 
    \begin{pmatrix}
        \textbf{u}_r\\
        \textbf{b}
    \end{pmatrix}
\end{align*}
The tensors $\textbf{U}^{(n)}_{o/i}$ (resp. $\textbf{P}^{(n)}_{o/i}$) are $(n+1)^{th}$ (resp. $n^{th}$) order tensors, solely function of \textbf{r} and the viscosity ratio $\lambda$. 
The tensors $\textbf{U}_{o/i}^{(1)}$ and $\textbf{P}_{o/i}^{(1)}$ represent the functional form of the famous Hadamard-Ribczynski solution \citep{pozrikidis1992boundary,kim2013microhydrodynamics}. 
The dependency of $\textbf{u}_{i/o}$ and $p_{i/o}$ with the mean gradient velocity $\grad \textbf{u}$ is given by the tensor $\textbf{U}_{o/i}^{(2)}$ and $\textbf{P}_{o}^{(2)}$.
The disturbance velocity and pressure fields of a drop immersed in pure linear flow can be found in \citet{rallison1978note,leal2007advanced,raja2010inertial}. 
Finally, the disturbance field of a droplet immersed in a pure quadratic flow is defined through the tensor $\textbf{U}_{o/i}^{(3)}$ and $\textbf{P}_{o/i}^{(3)}$.
The definition of the former tensors may be found in \citet{nadim1991motion}.




The tensors $\textbf{U}^{(b-n)}_{o/i}$ (resp. $\textbf{P}^{(b-n)}_{o/i}$) are $(n+1)^{th}$ (resp. $n^{th}$) order tensors, solely function of \textbf{r} and the viscosity ratio $\lambda$ as well. 
The disturbance fields induced due to a constant, linear, or quadratic stress jump at the interface of the droplet is less common in the literature. 
For instance one might refer to \citet{Subramanian_1985,leal2007advanced} to compute the disturbance fields due to a constant surface tension gradient, hence defining the expression of  $\textbf{U}_{o/i}^{(b-1)}$ and $\textbf{P}_{o/i}^{(b-1)}$. 
Then to express the disturbance fields in terms of $\grad \textbf{b}$ or higher order derivatives one might refer to the solution given in \citet[Appendix C]{raja2010inertial}.
Without loss of generality we consider only the symmetric traceless part of $(\grad \textbf{b}_{jk})$ in the following. 
Based on the classic method of spherical harmonic \citep[chapter 8]{leal2007advanced} we could derive the expression for the disturbance fields due to an imposed $\grad\grad \textbf{b}$, it reads,
\begin{align*}
    (\textbf{U}_o^{(b-3)})_{ijkl}
    &=
    -\frac{7r^4+10r^2-9}{1260(\lambda+1)r^5}(
        \delta_{ij}\delta_{kl}
        + \delta_{ik}\delta_{jl}
        + \delta_{il}\delta_{kj}
        )
    -\frac{7r^4-60r^2+45}{1260(\lambda+1)r^7}(
        x_ix_j\delta_{kl}
        + x_ix_k\delta_{jl}
        + x_ix_l\delta_{kj}
        )\\
    &+ \frac{r^2 -3}{84(\lambda +1)r^7}(
        \delta_{ij}x_kx_l
        + \delta_{ik}x_jx_l
        + \delta_{il}x_kx_j
    )
    - \frac{5r^2 - 7}{28(\lambda+1)r^9}x_ix_jx_kx_l
    \\
    (\textbf{P}_o^{(b-3)})_{jkl}
    &=
    -\frac{7r^2 - 45}{630(\lambda+1)r^5}(
        \delta_{jk}x_l
        + \delta_{jl}x_k
        + \delta_{lk}x_j
    )
    - \frac{5}{14(\lambda+1)r^7}x_jx_kx_l
    \\
    (\textbf{U}_i^{(b-2)})_{ijk}
    &=
    \frac{9r^4-20r^2+7}{630(\lambda+1)}(
        \delta_{ij}\delta_{kl}
        + \delta_{ik}\delta_{jl}
        + \delta_{il}\delta_{kj}
    )
    +\frac{9r^2-5}{630(\lambda+1)}(
        x_ix_j\delta_{kl}
        + x_ix_k\delta_{jl}
        + x_ix_l\delta_{kj}
        )\\
    &- \frac{3r^2-2}{42(\lambda +1)}(
        \delta_{ij}x_kx_l
        + \delta_{ik}x_jx_l
        + \delta_{il}x_kx_j
    )
    + \frac{1}{14(\lambda+1)}x_ix_jx_kx_l
    \\
    (\textbf{P}_i^{(b-3)})_{jkl}
    &=
    +\frac{54r^2 - 35}{315(\lambda+1)r}(
        \delta_{jk}x_l
        + \delta_{jl}x_k
        + \delta_{lk}x_j
    )
    - \frac{6}{7(\lambda+1)}x_jx_kx_l. 
\end{align*}
It is implied that each of these tensors must be contracted with the full symmetric tensor $(\grad\grad\textbf{b})_{ijk} \sim (\grad\grad\grad\gamma)_{ijk}$ to obtain the velocity or pressure fields. 

Hence, based on these expressions and the solutions  provided in the literature, one can compute the force traction at the surface of the droplet ($\bm\sigma_{out}\cdot \textbf{n}$), as well as the internal shear rate ($\textbf{e}_{in}$), and obtains the following expressions, 
\begin{align}
    \intS{\bm\sigma_{out}\cdot \textbf{n}} &
    =
    2\pi\frac{2+3\lambda}{1+\lambda}\textbf{u}_r
    + \pi \frac{\lambda}{\lambda +1} \grad^2 \textbf{u}
    +
    \frac{4\pi}{3}\frac{1}{\lambda +1}\textbf{b}
    + \frac{2\pi}{15(\lambda +1)}\grad^2\textbf{b}
    \\
    \intS{ \textbf{x}\bm\sigma_{out}\cdot \textbf{n}} &
    =
    \frac{2\pi(5\lambda +2)}{5(\lambda +1)}[\grad \textbf{u}+ (\grad \textbf{u})^\dagger]
    + \frac{12\pi}{25(\lambda +1)} \grad \textbf{b} 
    \\
    \intS{\textbf{xx}\bm\sigma_{out}\cdot \textbf{n}} &
    =
    \frac{4\pi}{5(\lambda +1)} (\textbf{u}_r \bm\delta + ^\dagger\textbf{u}_r \bm\delta)
    + \frac{2\pi(5\lambda +2)}{5(\lambda+1)}\bm\delta \textbf{u}_r
    - \frac{8\pi}{15(\lambda +1)} ( \textbf{b}\bm\delta + ^\dagger\textbf{b}\bm\delta )
    + \frac{4\pi}{5(\lambda+1)}\bm\delta \textbf{b}
    \label{eq:nd_mom}
\end{align}
and, 
\begin{align}
    \intO{2\textbf{e}_{in}}
    &=
    -\frac{4\pi}{15}\frac{5\lambda +2}{\lambda+1}
    [\grad \textbf{u}+ (\grad \textbf{u})^\dagger]
    - \frac{8\pi}{25}\frac{1}{\lambda+1}
    \grad\textbf{b}
    % + \frac{8\pi}{75}\frac{1}{\lambda+1}
    % \bm\delta\div \textbf{b}
    \\
    \intO{2\textbf{r}\textbf{e}_{in}}
    &=
    \frac{2\pi}{5(\lambda+1)}
    (\bm\delta \textbf{u}_r +  \bm\delta\textbf{u}_r^\dagger)
    -\frac{4\pi}{15(\lambda+1)}\textbf{u}_r\bm\delta 
    -\frac{4\pi}{15}\frac{1}{\lambda+1}
    (\bm\delta \textbf{b} +  \bm\delta\textbf{b}^\dagger)
    +\frac{8\pi}{45}\frac{1}{\lambda+1}
    \textbf{b}\bm\delta. 
    \label{eq:st_mom}
\end{align}
In these expressions we did not include the dependence on $\propto \grad\grad \textbf{u}$ and $\propto \grad\grad \textbf{b}$ in \ref{eq:nd_mom} and \ref{eq:st_mom} because they turn out to be of $O(a^2/L^2)$, hence negligible in the averaged equation. 
Nevertheless, they will be needed to compute the deformation of the droplets, hence we display here the higher order terms, namely 
\begin{multline}
    \intS{(\textbf{xx})_{jk}(\bm\sigma_{out}\cdot \textbf{n})_i} 
    =
    \frac{7\lambda^2+190\lambda+88}{105(\lambda^2+5\lambda+4)}[
        (\grad\grad \textbf{u})_{ijk}
        + (\grad\grad \textbf{u})_{ikj}
    ]
    + \frac{119\lambda^2+190\lambda-24}{105(\lambda^2+5\lambda+4)}(\grad\grad \textbf{u})_{jki}\\
    - \frac{7\lambda^2+80\lambda-72}{105(\lambda^2+5\lambda+4)}[
        (\bm\delta \grad^2 \textbf{u})_{ijk}
        + (\bm\delta \grad^2 \textbf{u})_{ikj}
    ]
    + \frac{2(13\lambda-4)}{21(\lambda^2+5\lambda+4)}(\bm\delta\grad^2 \textbf{u})_{jki}\\
    \frac{76}{735(\lambda+1)}(\grad\grad \textbf{b})_{ijk}
    + \frac{218}{3675(\lambda+1)} (\bm\delta\grad^2\textbf{b})_{jki}
    - \frac{272}{3675(\lambda+1)} [(\bm\delta\grad^2\textbf{b})_{ijk}+(\bm\delta\grad^2\textbf{b})_{ikj}],
    \label{eq:second_order_closuresS}
\end{multline}
\begin{multline}
    \intS{(\textbf{x})_{k}(\textbf{e}_{in})_{ij}} 
    =
    - \frac{7\lambda^2+20\lambda+3}{105(\lambda^2+5\lambda+4)}[
        (\grad\grad \textbf{u})_{kij}
        + (\grad\grad \textbf{u})_{kji}
    ]
    - \frac{8(2\lambda+1)}{21(\lambda^2+5\lambda+4)}(\grad\grad \textbf{u})_{ijk}\\
    - \frac{\lambda-10}{21(\lambda^2+5\lambda+4)}[
        (\bm\delta \grad^2 \textbf{u})_{jki}
        + (\bm\delta \grad^2 \textbf{u})_{ikj}
    ]
    + \frac{2(3\lambda-2)}{21(\lambda^2+5\lambda+4)}(\bm\delta\grad^2 \textbf{u})_{ijk}\\
    - \frac{32}{735(\lambda+1)}(\grad\grad \textbf{b})_{ijk}
    + \frac{292}{11025(\lambda+1)} (\bm\delta\grad^2\textbf{b})_{ijk}
    - \frac{22}{1225(\lambda+1)} [(\bm\delta\grad^2\textbf{b})_{jki}+(\bm\delta\grad^2\textbf{b})_{ikj}].
    \label{eq:second_order_closuresE}
\end{multline}


\subsubsection*{Deformation of the droplets}

In the body of the text we use the second moment of momentum equation to determine the third mode of deformation and show that it is negligible. 
Here we provide additional information on the derivation of the second moment of momentum equation. 
Based on the general formula \ref{eq:dt_Q_n} one obtain by neglecting the inertial effects  and the body forces,  
\begin{equation}
    \intO{ r_{j}(\bm{\sigma}^0_d)_{ik}+r_{k}(\bm{\sigma}^0_d)_{ji}}
    +\intS{ r_{j}(\bm{\sigma}^0_\Gamma)_{ik}+r_{k}(\bm{\sigma}_\Gamma^0)_{ji}}
    = 
    \intS{  r_{k}r_{j} (\bm{\sigma}_f^0\cdot\textbf{n})_i }
    % + \intO{ r_{k}r_{j}  \rho_d (\textbf{b}_d^0)_i }.  
    \label{eq:step_1}
\end{equation}
% the mean part of the stress then read
% \begin{equation}
%     \ldots=\intO{  r_{k}r_{j} (\div \bm{\Sigma})_i }
%     +(1-\lambda)\intS{  (\bm{\Sigma})_{ik} r_{j}  }
%     +(1-\lambda)\intS{  (\bm{\Sigma})_{ij} r_{k}  }
% \end{equation}
Using the trick of \citet{lhuillier1996contribution} we may re-write this equation by summing and subtracting the permutations:  $B_{ijk} + B_{jik} - B_{kij}$, where $B_{ijk}$ corresponds to \ref{eq:step_1}. 
This gives, 
\begin{align}
    \intO{2 r_{k}(\bm{\sigma}^0_d)_{ij}}
    +\intS{2\gamma r_{k}(\bm\delta - \textbf{nn})_{ij}}
    &= 
    +\intS{
        r_{k}r_{j} (\bm{\sigma}_f^0\cdot\textbf{n})_i 
        + r_{k}r_{i} (\bm{\sigma}_f^0\cdot\textbf{n})_j 
        - r_{j}r_{i} (\bm{\sigma}_f^0\cdot\textbf{n})_k 
    }
    % \\
    % &
    % + \intO{ 
    %     r_{k}r_{j}  \rho_d (\textbf{b}_d^0)_i 
    %     +r_{k}r_{i}  \rho_d (\textbf{b}_d^0)_j 
    %     -r_{j}r_{i}  \rho_d (\textbf{b}_d^0)_k 
    %     }
    % \label{eq:dt_P2_alpha_bis}
\end{align}
Taking the traceless part of this equation on the index $ij$, and substituting $\bm\sigma_f^0 \to \bm\sigma_f^* + \bm\Sigma$ and $\textbf{e}_d^0 \to \textbf{e}_d^* + \textbf{E}$ one obtains, 
% \begin{align}
%     \intO{2 r_{k}(\bm{\sigma}^0_d)_{ij}^{dev}}
%     +\intS{2r_{k}(\bm{\sigma}^0_\Gamma)_{ij}^{dev}}
%     &= 
%     +\intS{
%         r_{k}r_{j} (\bm{\sigma}_f^0\cdot\textbf{n})_i 
%         + r_{k}r_{i} (\bm{\sigma}_f^0\cdot\textbf{n})_j 
%         - r_{j}r_{i} (\bm{\sigma}_f^0\cdot\textbf{n})_k 
%     }\\
%     &-\frac{1}{3}\delta_{ij}\intS{
%         r_{k}r_{l} (\bm{\sigma}_f^0\cdot\textbf{n})_l
%         + r_{k}r_{l} (\bm{\sigma}_f^0\cdot\textbf{n})_l 
%         - r_{l}r_{l} (\bm{\sigma}_f^0\cdot\textbf{n})_k 
%     }\\
%     &+\intO{  
%         r_{k}r_{j} (\div \bm{\Sigma})_i 
%         +r_{k}r_{i} (\div \bm{\Sigma})_j 
%         -r_{j}r_{i} (\div \bm{\Sigma})_k 
%         }\\
%     &-\frac{1}{3}\delta_{ij}\intO{  
%         r_{k}r_{l} (\div \bm{\Sigma})_l
%         +r_{k}r_{l} (\div \bm{\Sigma})_l 
%         -r_{l}r_{l} (\div \bm{\Sigma})_k 
%         }\\
%     &+\mu_f (1-\lambda)\intS{ 4\textbf{E}_{ij} r_{k}  }
%     \\
%     &
%     + \rho_d \intO{ 
%         r_{k}r_{j} (\textbf{b}_d^0)_i 
%         +r_{k}r_{i} (\textbf{b}_d^0)_j 
%         -r_{j}r_{i} (\textbf{b}_d^0)_k 
%         }\\
%     &-\rho_d \frac{1}{3}\delta_{ij} \intO{ 
%         r_{k}r_{l} (\textbf{b}_d^0)_l 
%         +r_{k}r_{l} (\textbf{b}_d^0)_l 
%         -r_{l}r_{l} (\textbf{b}_d^0)_k 
%         }
%     % \label{eq:dt_P2_alpha_bis}
% \end{align}
\begin{align}
    \intS{2\gamma r_{k}(\bm\delta/3 - \textbf{nn})_{ij}}
    &= 
    +\intS{
        r_{k}r_{j} (\bm{\sigma}^*_f\cdot\textbf{n})_i 
        + r_{k}r_{i} (\bm{\sigma}^*_f\cdot\textbf{n})_j 
        - r_{j}r_{i} (\bm{\sigma}^*_f\cdot\textbf{n})_k 
    }\nonumber \\
    &-\frac{1}{3}\delta_{ij}\intS{
        r_{k}r_{l} (\bm{\sigma}^*_f\cdot\textbf{n})_l
        + r_{k}r_{l} (\bm{\sigma}^*_f\cdot\textbf{n})_l 
        - r_{l}r_{l} (\bm{\sigma}^*_f\cdot\textbf{n})_k 
    }\nonumber \\
    &+\mu_f (1-\lambda)\intS{ 4\textbf{E}_{ij} r_{k}  }
    - \mu_f\lambda \intO{2 r_{k}(\textbf{e}_d^*)_{ij}}
    % \\
    % &
    % + (\rho_d-\rho_f) \intO{ 
    %     r_{k}r_{j} \textbf{g}_i 
    %     +r_{k}r_{i} \textbf{g}_j 
    %     -r_{j}r_{i} \textbf{g}_k 
    %     }\\
    % &-(\rho_d-\rho_f) \frac{1}{3}\delta_{ij} \intO{ 
    %     r_{k}r_{l} \textbf{g}_l 
    %     +r_{k}r_{l} \textbf{g}_l 
    %     -r_{l}r_{l} \textbf{g}_k 
    %     }
    \label{eq:second_mom}
\end{align}
where we have noticed that $ \div\bm\Sigma = -  \rho_f \textbf{g}$ at $O(1)$ in $\phi$, and because we neglected the body forces in this example  $\div\bm\Sigma =0$. 
Injecting \ref{eq:second_order_closuresS,eq:second_order_closuresE} in \ref{eq:second_mom} one arrive at \ref{eq:defH3}.


